<section xml:id="sec-">
    <title>Logical Axioms</title>
    
    <p>
    Our formal concept of proof is grounded in standard first order logic with an equality symbol. For definitiveness,
    we will assume the following axioms and rules of inference:
    </p>
    <definition xml:id="def-FOL">
        <title>Logical Axioms</title>
        <statement>
            <p>
            We assume the following logical axioms
            </p>
            <ol>
                <li>
                    <p>
                    <m> \phi\rightarrow(\psi\rightarrow\phi)</m>
                    </p>
                </li>
                <li>
                    <p>
                        <m>(\phi\rightarrow (\psi\rightarrow\eta))\rightarrow((\phi\rightarrow\psi)\rightarrow(\phi\rightarrow\eta)).</m>
                    </p>
                </li>
                <li>
                    <p>
                        <m>(\neg\phi\rightarrow\neg\psi)\rightarrow(\psi\rightarrow\phi)</m>    
                    </p>
                </li>
                <li>
                    <p>
                        <m>(\forall x)(\phi\rightarrow\psi)\rightarrow(\phi\rightarrow(\forall x)\psi)</m> where <m>x</m> is not free in <m>\phi</m>.    
                    </p>
                </li>
                <li>
                    <p>
                        <m>(\forall x)\phi(x)\rightarrow\phi(y)</m> where <m>x</m> has no free occurrence in a subformula of form <m>(\forall y)\psi</m>.
                    </p>
                </li>
            </ol>
        </statement>
    </definition>
<p> The rules of inference we adopt are as follows:</p>
<ul>
    <li>
        <p>
            <m>\psi</m> follows from <m>\phi</m> and <m>\phi\rightarrow\psi</m>, and
        </p>
    </li>
    <li>
        <p>
            <m>(\forall x)\phi</m> follows from <m>\phi</m>.    
        </p>
    </li>
</ul>
</section>